\documentclass{article}
\input{preamble.tex}

% Title
\title{12.4 Composition}
\author{Benjamin Basseri}


\begin{document}

\maketitle

\begin{problem}
Suppose $A = \{5, 6, 8\}$, $B = \{0, 1\}$, $C = \{1, 2, 3\}$. Let $f : A \to B$ be the function $f = \{(5, 1), (6, 0), (8, 1)\}$, and $g : B \to C$ be $g = \{(0, 1), (1, 1)\}$. Find $g \circ f$.
\end{problem}

We can go through the domain of $f$ and its mappings through $g$ or notice that $g$ is the constant 1 function, so the set presentation of $f$ is:
$$f = \{(5, 1), (6, 1), (8, 1)\}$$

\begin{problem}
Suppose $A = \{1, 2, 3, 4\}$, $B = \{0, 1, 2\}$, $C = \{1, 2, 3\}$. Let $f : A \to B$ be $f = \{(1, 0), (2, 1), (3, 2), (4, 0)\}$, and $g : B \to C$ be $g = \{(0, 1), (1, 1), (2, 3)\}$. Find $g \circ f$.
\end{problem}

$$f(1) = 0, g(0) = 1 \implies g(f(1)) = 1$$
$$f(2) = 1, g(1) = 1 \implies g(f(2)) = 1$$
$$f(3) = 2, g(2) = 3 \implies g(f(3)) = 3$$
$$f(4) = 0, g(0) = 1 \implies g(f(4)) = 1$$

$$g\circ f = \{(1, 1), (2, 1), (3, 3), (4, 1)\}$$

\begin{problem}
Suppose $A = \{1, 2, 3\}$. Let $f : A \to A$ be the function $f = \{(1, 2), (2, 2), (3, 1)\}$, and let $g : A \to A$ be the function $g = \{(1, 3), (2, 1), (3, 2)\}$. Find $g \circ f$ and $f \circ g$.
\end{problem}

$$f(1) = 2, g(2) = 1 \implies g(f(1)) =1$$
$$f(2) = 2, g(2) = 1 \implies g(f(2)) = 1$$
$$f(3) = 1, g(1) = 3 \implies g(f(3)) = 3$$
$$g\circ f = \{(1, 1), (2, 1), (3, 3)\}$$

$$g(1) = 3, f(3) = 1 \implies f(g(1)) = 1$$
$$g(2) = 1, f(1) = 2 \implies f(g(2)) = 2$$
$$g(3) = 2, f(2) = 2 \implies f(g(3)) = 2$$
$$f\circ g = \{(1, 1), (2, 2), (3, 2)\}$$

\begin{problem}
Suppose $A = \{a, b, c\}$. Let $f : A \to A$ be the function $f = \{(a, c), (b, c), (c, c)\}$, and let $g : A \to A$ be the function $g = \{(a, a), (b, b), (c, a)\}$. Find $g \circ f$ and $f \circ g$.
\end{problem}

$$f(a) = c, g(c) = a \implies g(f(a)) = a$$
$$f(b) = c, g(c) = a \implies g(f(b)) = a$$
$$f(c) = c, g(c) = a \implies g(f(c)) = a$$
$$g \circ f = \{(a, a), (b, a), (c, a)$$

For $f \circ g$ we only need notice that $f$ is the constant $c$ function, so any input $g$ provides, $f \circ g$ also maps to $c$ and is the contstant $c$ function.

\begin{problem}
Consider the function $f, g: \R \to \R$ defined as $f(x) = \sqrt[3]{x+1}$ and $g(x) = x^3$. Find the formulas for $g \circ f$ and $f \circ g$.
\end{problem}

$$(g \circ f)(x) = g(f(x)) = g(\sqrt[3]{x + 1}) = \left(\sqrt[3]{x+1}\right)^3 = x + 1$$
$$(f \circ g)(x) = f(g(x)) = f(x^3) = \sqrt[3]{x^3 + 1}$$

\begin{problem}
Consider the functions $f, g: \R \to \R$ defined as $f(x) = \frac{1}{x^2 + 1}$ and $g(x) = 3x + 2$. Find the formulas for $g \circ f$ and $f\circ g$.
\end{problem}

$$(g \circ f)(x) = g(f(x)) = g\left(\frac{1}{x^2 + 1}\right) = \frac{3}{x^2 + 1} + 2$$
$$(f \circ g)(x) = f(g(x)) = f(3x+2) = \frac{1}{(3x + 2)^2 + 1} = \frac{1}{9x^2 + 12x + 5}$$

\begin{problem}
Consider the functions $f, g: \Z \times \Z \to \Z \times \Z$ defined as $f(m, n) = (mn, m^2)$ and $g(m, n) = (m + 1, m + n)$. Find the formulas for $g \circ f$ and $f \circ g$.
\end{problem}

$$(g \circ f)(m, n) = g(f(m, n)) = g(mn, m^2) = (mn + 1, mn + m^2)$$
$$(f \circ g)(m, n) = f(g(m, n)) = f(m + 1, m + n) = ((m+1)(m + n), (m + 1)^2) = (m^2 + mn + m + n, m^2 + 2m + 1)$$

\begin{problem}
Consider the functions $f, g: \Z \times \Z \to \Z \times \Z$ defined as $f(m, n) = (3m - 4n,m 2m + n)$ and $g(m, n) = (5m +n, m)$. Find the formulas for $g\circ f$ and $f\circ g$.
\end{problem}

$$(g\circ f)(m, n) = g(f(m, n)) = g(3m-4n, 2m +n) = (5(3m - 4n) + (2m + n), 3m - 4n) = (17m -19n, 3m -4n)$$
$$(f\circ g)(m, n) = f(g(m, n)) = f(5m+n, m) = (3(5m + n) - 4m, 2(5m+n) + m) = (11m + 3n, 11m + 2n)$$

\begin{problem}
Consider the functions $f:\Z \times \Z \to \Z$ defined as $f(m,n) = m+n$ and $g: \Z \to \Z \times \Z$ defined as $g(m) = (m, m)$. Find the formulas for $g\circ f$ and $f\circ g$
\end{problem}

$$(g\circ f)(m, n) = g(f(m, n)) = g(m +n) = (m+n, m+n)$$
$$(f \circ g)(m) = f(g(m)) = f(m, m) = (2m, 2m)$$

\begin{problem}
Consider the function $f: \R^2 \to \R^2$ defined by the formula $f(x, y) = (xy, x^3).$ Find a formula for $f\circ f$.
\end{problem}

$$(f \circ f)(x, y) = f(xy, x^3) = ((xy)x^3, (xy)^3) = (x^4 y, x^3 y^3)$$

\end{document}
